\documentclass{report}
\usepackage{amsmath}
\usepackage{geometry}
\usepackage{amssymb}
 \geometry{
 a4paper,
 total={170mm,257mm},
 left=20mm,
 top=20mm,
 }
\title{\fontsize{40}{48} \selectfont \textbf{Mathematical Notes \\  2018}}
\author{\textbf{L. L.H. Lau}}
\date{}


\begin{document}
\maketitle
\chapter*{Groups}
\vspace{10.0mm}
\section*{Group Axioms}
\large{ A group G is a set G with a binary operation denoted by $\bullet$  which satisfies the following axioms:\\ 
\begin{enumerate}
	\item \textbf{Identity}\\
		\linebreak
		$\forall$ a $\in$ G, $\exists$ e $\in$ G, s.t. e $\bullet$ a = a $\bullet$ e = a   
	\item \textbf{Inverse}\\
		\linebreak
		 $\forall$ a $\in$ G, $\exists$ $a^{-1}$ $\in$ G, s.t. $a^{-1}$ $ \bullet$ a = a $\bullet$ $a^{-1}$ = e
	\item \textbf{Associativity}\\
		\linebreak
		$\forall$ a, b, c $\in$ G, a $\bullet$ (b $\bullet$ c) = (a $\bullet$ b) $\bullet$ c
	\item \textbf{Closure}\\
		\linebreak
		$\forall$ a, b $\in$ G, (a $\bullet$ b) $\in$ G	
\end{enumerate}


}

\section*{Order}
\large{
	The order of a group G is denoted $\|$ G $\|$ and gives the number of elements in G. 
\\	The order of an element g $\in$ G, denoted by n, is the smallest integer n such that $g^{n}$ = e.
	It is trivial to see that ord(e) = 1 and if an element t $\in$ G is self inverse, ord(t) = 2.

\subsection*{Proof that the order of g \& $g^{-1}$ are the same}
	Let $n_1$ be s.t. $g^{n_1}$ = e and $n_1$ is the smallest such integer.
	\begin{alignat*}{2}
		&(g^{-1}g) &&= e \\
		\implies &(g^{-1}g)^{n_1} &&= e^{n_1} = e\\
		\implies &(g^{-1})^{n_1}g^{n_1} &&= e\\ 
		\implies &(g^{-1})^{n_1} &&= e
	\end{alignat*}
	Here $n_1$ is a multiple of the smallest such integer for $g^{-1}$. Similarly we can define the smallest integer $n_2$ 
	which satisfies $(g^{-1})^{n_2} = e$ . By symmetry we get $n_1$ and $n_2$ being multiples of each other. $\therefore n_1 = n_{2}$
	\newpage

\subsection*{Exercises \\}
	\begin{enumerate}
	\item Proof of the uniqueness of the identity and the inverse.\\
	\item Prove that  $\forall$ a, b $\in G$ $ord(ba) = ord(ab)$.
	\end{enumerate}

}

\section*{Types of Groups}
\large{
	\subsection*{Abelian Groups}
		A group G is abelian if it follows the group axioms and also has a commutativity axiom. Where $\forall$ a, b $\in G$ $a \bullet b = b \bullet a$ .  
	\subsection*{Cyclic Group}
		For a cyclic group G of order n, all emements of the group can be generated from one element of the group, e.g. X.
		\begin{equation*}
			G = \{I, X, X^2, X^3, ... , X^{n-1}\}
		\end{equation*}
		A cyclic group is abelian and all elements of G, apart from I have order n, the same as the ord(G) - the number of elements in group G.
	\section*{Subgroup}
		A group H is a subgroup of G, denoted by $H \leq G$, \textbf{iff} the set H is a subset of the set G, denoted by $H \subseteq G$, and follows the group axioms.
		This can be summarised by the following, where the group H is a non empty set with a binary operator $\bullet$ : 
		\begin{equation*}
			\forall a, b \in H, (ab^{-1})\in H	
		\end{equation*}
		The logic follows as such:
		\begin{alignat*}{2}
			& a \in H \\
			&aa^{-1}\in H &&\implies e \in H \text{ (By substitution of b for a- identity axiom)} \\
			&ea^{-1}\in H &&\implies a^{-1} \in H \text{(Inverse Axiom)}\\ 
			&b \in H &&\implies b^{-1} \in H \therefore a(b^{-1})^{-1} \in H \implies ab \in H \text{(Closure)}
		\end{alignat*}
}

\chapter*{List of Common DEs} 
\vspace{10.0mm}
\section*{First Order ODEs}
\large{
\subsection*{\textbf{Separable:}}
	 $\frac{dy}{dx} = f(x)g(y)$ \\ \\ If you can't do this, just give up.

\subsection*{\textbf{Exact:}} $A(x,y)dx + B(x,y)dy = 0$ and $\frac{\partial A}{\partial y} = \frac{\partial B}{\partial x}$ \\ \\This follows from the symmetry of mixed partial derivatives.
\\ To find the function U which satisfies $\frac{\partial U}{\partial x} = A$ and $\frac{\partial U}{\partial y} = B$ we can take the union of the generalised functions solved by integrating. Remember due to the partial derivatives we get some functions of x or y instead of constants of integration.

\subsection*{\textbf{Inexact:}} $A(x,y)dx + B(x,y)dy = 0$ and $\frac{\partial A}{\partial y} \neq \frac{\partial B}{\partial x}$






}

\end{document}
